Continuation.v
@@ -1,0 +1,876 @@
+(* *)
+
+Require Import Norm.
+Require Import Rewrites.
+Require Import Term.
+Require Import Omega.
+
+Inductive Continuation :=
+  Empty : Continuation
+| Iterate : Term -> Continuation -> Continuation.
+
+Fixpoint plug (K : Continuation) (M : Term) : Term :=
+  match K with
+      Empty => M
+    | Iterate N K' => plug K' (TmBind M N)
+  end.
+
+(* Inductive Krw_explicit : Continuation -> Continuation -> Type := *)
+(* | A : forall N N' K, (N ~> N') -> Krw_explicit (Iterate N K) (Iterate N' K) *)
+(* | B : forall N K K', (Krw_explicit K K') -> Krw_explicit (Iterate N K) (Iterate N K') *)
+(* . *)
+
+Definition SNK (K : Continuation) :=
+  forall M,
+    SN M ->
+    SN (plug K (TmSingle M)).
+
+Definition ReducibleK (Reducible:Term->Ty -> Type) (K : Continuation) (T : Ty) :=
+    forall M,
+      Reducible M T ->
+      SN (plug K (TmSingle M)).
+
+Lemma plug_SN_rw:
+  forall K M M',
+    (M ~> M') -> SN (plug K M) -> SN (plug K M').
+Proof.
+ induction K.
+  simpl.
+  intuition.
+  inversion H0.
+  auto.
+ simpl.
+ intros.
+ apply IHK with (TmBind M t); sauto.
+Qed.
+
+(* Lemma KM_rw_inversion: *)
+(*   forall K M km', *)
+(*     (plug K M ~> km') -> {M' : Term & km' = plug K M'}. *)
+(* Proof. *)
+ 
+(* Qed. *)
+
+Lemma rw_plug_lift :
+  forall K M M',
+    (M ~> M') -> (plug K M ~> plug K M').
+Proof.
+ induction K.
+  auto.
+  simpl.
+ intros.
+ apply IHK.
+ auto.
+Qed.
+
+Definition HoleType K T :=
+  forall M env, Typing env M T -> {S : Ty & Typing nil (plug K M) S}.
+
+Definition Krw K K' := (forall M, plug K M ~> plug K' M).
+
+(** Reflexive, transitive closure of Krw *)
+Inductive Krw_rt : Continuation -> Continuation -> Type :=
+| Krw_rt_refl : forall m n, m = n -> Krw_rt m n
+| Krw_rt_step : forall m n, Krw m n -> Krw_rt m n
+| Krw_rt_trans : forall l m n, Krw_rt l m -> Krw_rt m n
+                -> Krw_rt l n.
+
+(* Inductive SNK K := *)
+(*   Reducts_SNK : (forall K', Krw K K' -> SNK K') -> SNK K. *)
+
+(* Lemma Krw_Iterate: *)
+(*   forall K K' t, *)
+(*     Krw K K'-> Krw (Iterate t K) (Iterate t K'). *)
+(* Proof. *)
+(*  induction K; simpl. *)
+(*   unfold Krw. *)
+(*   intros. *)
+(*   simpl in *. *)
+(*   assert (K' = Empty). *)
+  
+(*   assert (TmBind M t ~> TmBind (plug K' M) t). *)
+(*    apply Rw_Bind_subject. *)
+(*    auto. *)
+
+(* Qed. *)
+
+Lemma iterate_reduce K K' : Krw K K' -> forall F, Krw (Iterate F K) (Iterate F K').
+Proof.
+unfold Krw.
+intros.
+simpl.
+apply H.
+Qed.
+
+Lemma Rw_under_K:
+  forall K M N,
+    (M ~> N) -> (plug K M ~> plug K N).
+Proof.
+ induction K; simpl; intros.
+  auto.
+ apply IHK.
+ auto.
+Qed.
+
+Lemma rw_in_K_body:
+  forall K M M',
+   (M ~> M') -> (Krw (Iterate M K) (Iterate M' K)).
+Proof.
+ intros.
+ unfold Krw.
+ intros.
+ simpl.
+ apply Rw_under_K.
+ eauto.
+Qed.
+
+Lemma Krw_SNK K K' : SNK K -> Krw K K' -> SNK K'.
+Proof.
+ unfold SNK, Krw in *.
+ intros.
+ specialize (H M H1).
+ inversion H.
+ auto.
+Qed.
+
+Lemma Krw_rt_SNK K K' : SNK K -> Krw_rt K K' -> SNK K'.
+Proof.
+ intros.
+ induction H0.
+   subst; auto.
+  eauto using Krw_SNK.
+ auto.
+Qed.
+
+Lemma plug_SN_rw_rt:
+  forall (K : Continuation) (M M' : Term),
+  (M ~>> M') -> SN (plug K M) -> SN (plug K M').
+Proof.
+ intros.
+ induction H; subst; eauto using plug_SN_rw.
+Qed.
+
+Lemma Empty_unrewritable: forall K, (Krw Empty K) -> False.
+Proof.
+ unfold Krw.
+ intros.
+ specialize (H TmConst).
+ destruct K; simpl in H; inversion H.
+Qed.
+
+Inductive Ktyping : Continuation -> Ty -> Type :=
+  Ktype : forall K T env S M, Typing env M T -> Typing nil (plug K M) S -> Ktyping K T.
+
+Lemma Krw_characterization:
+  forall K T K' N,
+    Ktyping K T ->
+    Krw (Iterate N K) K' ->
+    {K1 : Continuation & ((K' = Iterate N K1) * (Krw K K1))%type} +
+    {N' : Term & ((K' = Iterate N' K) * (N ~> N'))%type}.
+Proof.
+Admitted  (* unused *).
+
+Lemma SN_push_under_k:
+  forall K M,
+    SN (plug K M) ->
+    SN M.
+Proof.
+ induction K.
+  simpl.
+  auto.
+ intros.
+ simpl in H.
+ pose (s := IHK (TmBind M t) H).
+ eapply SN_embedding with (f := fun x => TmBind x t) (Q := TmBind M t); sauto.
+Qed.
+
+(* Induction on the reduction sequences of two objects: K and M.
+ Unused but might be good practice?
+*)
+Lemma double_induction_K P K M:
+  (forall M0,
+     (M ~>> M0) ->
+     Neutral M0 ->
+     (  (forall K', (Krw K K') -> P K' M0)
+      -> (forall M', (M0 ~> M') -> P K M')
+      -> P K M0))
+  ->
+  forall plug_K_M, (plug K M ~>> plug_K_M) ->
+                   Neutral M ->
+                   SN plug_K_M -> P K M.
+Proof.
+(* Idea: Use SN_embedding's approach instead. *)
+Admitted.
+
+Lemma Neutral_Lists:
+  forall K M,
+    Neutral M ->
+    forall Z, (plug K M ~> Z) ->
+    {M' : Term & ((Z = plug K M') * (M ~> M'))%type} +
+    {K' : Continuation & ((Z = plug K' M) * (Krw K K'))%type}.
+Proof.
+ induction K.
+ (* Case : empty K *)
+  left.
+  simpl.
+  firstorder.
+ (* Case : K starts with an iterator. *)
+ intros.
+ apply IHK in H0; try apply Neutral_TmBind.
+ destruct H0.
+ (* Case : redn of K@M' is inside M'. *)
+  destruct s as [x [H0 H1]].
+  apply TmBind_Neutral_reducts in H1; auto.
+  destruct H1 as [[M' [H1a H1b]] | [N' [H1a H1b]]].
+   left.
+   exists M'.
+   subst x.
+   sauto.
+  right.
+  exists (Iterate N' K).
+  subst.
+  simpl.
+  split.
+   auto.
+  apply rw_in_K_body; sauto.
+
+ (* Case : redn of K@M' in inside K. *)
+ right.
+ destruct s as [x [H0 H1]].
+ exists (Iterate t x).
+ simpl.
+ intuition.
+ apply iterate_reduce; sauto.
+Qed.
+
+Lemma K_TmNull_rw:
+  forall K Z,
+    (plug K TmNull ~> Z) ->
+    {K' : Continuation & { N : Term & ((Z = plug K' TmNull) * (K = (Iterate N K')))%type} } +
+    {K' : Continuation & ((Krw K K') * (Z = plug K' TmNull))%type}.
+Proof.
+ destruct K; simpl; intros Z H.
+  inversion H.
+ apply Neutral_Lists in H; [| auto].
+ destruct H as [[M' [Ha Hb]] | [K' [Ha Hb]]].
+  inversion Hb.
+    subst.
+    left.
+    exists K.
+    exists t.
+    sauto.
+   solve [inversion H2].
+  subst.
+  right.
+  exists (Iterate n' K).
+  split.
+   auto.
+   apply rw_in_K_body; sauto.
+  sauto.
+ right.
+ subst.
+ exists (Iterate t K').
+ simpl.
+ firstorder.
+Qed.
+
+Lemma Krw_inhabited:
+  Krw (Iterate (TmBind TmNull TmNull) Empty) (Iterate TmNull Empty).
+Proof.
+ unfold Krw.
+ intros.
+ simpl.
+ eauto.
+Qed.
+
+Fixpoint Ksize K :=
+  match K with
+      Empty => 0
+    | Iterate _ K' => S (Ksize K')
+  end.
+
+Lemma Ksize_induction P :
+  (forall K, Ksize K = 0 -> P K) ->
+  (forall n K', (forall K, Ksize K = n -> P K) ->
+                (Ksize K' = S n) ->
+                (P K')) ->
+  forall K,
+    P K.
+Proof.
+ intros H0 H_ind.
+ intros K.
+ pose (n := Ksize K).
+ assert (n = Ksize K) by auto.
+ clearbody n.
+ revert n K H.
+ induction n.
+  auto.
+ intros K H.
+ destruct K.
+  simpl in H; auto.
+ apply H_ind with (n:=n); sauto.
+Qed.
+
+Lemma Ksize_induction_strong P :
+  (forall K, (forall K', Ksize K' <  Ksize K -> P K') -> P K) ->
+   forall K, P K.
+Proof.
+ intros X.
+ cut (forall n, (forall K', Ksize K' <= n -> P K')).
+ eauto.
+ induction n.
+ - intros.
+   destruct K'; auto.
+   apply X.
+   simpl.
+   intros.
+   let T := type of H in absurd T.
+   omega.
+   auto.
+   simpl in H; exfalso ; omega.
+ - intros.
+   apply X.
+   intros.
+   destruct (le_gt_dec (Ksize K'0) n).
+   * apply IHn; auto.
+   * apply X.
+     intros.
+     assert (Ksize K'0 = S n) by omega.
+     assert (Ksize K'1 <= n) by omega.
+     apply IHn.
+     auto.
+(* Seems like the above is dodgy; proving it twice? *)
+Qed.
+
+Lemma Krw_to_Iterate:
+  forall K t K',
+  Krw K (Iterate t K') ->
+  {K0 : Continuation & { M : Term &
+     K = Iterate M K0 }}.
+Proof.
+ destruct K.
+  intros.
+  unfold Krw in H.
+  specialize (H TmNull).
+  simpl in *.
+  inversion H.
+ intros.
+ exists K.
+ exists t.
+ auto.
+Qed.
+
+Fixpoint appendK K1 K2 :=
+  match K1 with
+    | Empty => K2
+    | Iterate N K1' => Iterate N (appendK K1' K2)
+  end.
+
+Fixpoint deepest_K M :=
+match M with
+| TmBind M' N' =>
+  let (K, body) := deepest_K M' in
+  (appendK K (Iterate N' Empty), body)
+| _ => (Empty, M)
+end.
+
+(* Fixpoint drop_outermost K := *)
+(* match K with *)
+(* | Iterate t Empty => (t, Empty) *)
+(* | Iterate t K' => let (f, K'') := drop_outermost K' in *)
+(*                   (f, Iterate t K'') *)
+(* | Empty => (TmNull, Empty) *)
+(* end. *)
+
+(* Lemma deepest_K_spec3 : *)
+(*   forall K M, *)
+(*     notT {M' : Term & {N' : Term & M = TmBind M' N'}} -> *)
+(*     deepest_K (plug K M) = (K, M). *)
+(* Proof. *)
+(*  induction K using Ksize_induction_strong; destruct K; simpl; intros. *)
+(*  - destruct M; simpl; auto. *)
+(*    contradiction H0. *)
+(*    eauto. *)
+(*  - rewrite H. *)
+(* Qed. *)
+
+Lemma plug_appendK:
+  forall K M M',
+    plug (appendK K (Iterate M Empty)) M' = TmBind (plug K M') M.
+Proof.
+ induction K; simpl; auto.
+Qed.
+
+Lemma deepest_K_spec:
+  forall M K' M',
+    deepest_K M = (K', M') ->
+    plug K' M' = M.
+Proof.
+ induction M; simpl; intros; inversion H; auto.
+ pose (X := deepest_K M1).
+ assert (X = deepest_K M1) by auto.
+ destruct X.
+ rewrite <- H0 in H.
+ inversion H.
+ subst.
+ pose (IHM1 c M').
+ rewrite <- e; auto.
+ apply plug_appendK.
+Qed.
+
+Lemma appendK_Empty:
+  forall K, appendK K Empty = K.
+Proof.
+ induction K; simpl; auto.
+ rewrite IHK.
+ auto.
+Qed.
+
+Lemma appendK_assoc:
+  forall K1 K2 K3,
+    appendK (appendK K1 K2) K3 = appendK K1 (appendK K2 K3).
+Proof.
+ induction K1; simpl; auto.
+ intros.
+ rewrite IHK1.
+ auto.
+Qed.
+
+Lemma deepest_K_plug:
+  forall K,
+     forall M K' M',
+       deepest_K M = (K', M') ->
+       deepest_K (plug K M) = (appendK K' K, M').
+Proof.
+ induction K.
+ - simpl.
+   intros.
+   rewrite appendK_Empty.
+   auto.
+ - simpl.
+   intros.
+   rewrite IHK with (K':=appendK K' (Iterate t Empty))(M':=M').
+   * rewrite appendK_assoc.
+     simpl.
+     auto.
+   * simpl.
+     rewrite H.
+     auto.
+Qed.
+
+(* Lemma deepest_K_spec2 : *)
+(*   forall K M N, *)
+(*     {M' : Term & {K' : Continuation & *)
+(*       {f : Continuation->Continuation & *)
+(*        deepest_K (plug K (TmBind M N)) = (f K', M')} & *)
+(*        deepest_K (TmBind M N) = (Iterate N K', M')}}. *)
+(* Proof. *)
+(*  induction K. *)
+(*  - simpl. *)
+(*    intros. *)
+(*    set (X := deepest_K M). *)
+(*    destruct X as [K body]. *)
+(*    eauto. *)
+(*  - intros. *)
+(*    simpl. *)
+(*    pose (IHK (TmBind M N) t). *)
+(*    destruct s as [M' [K' [f Ha] Hb]]. *)
+(*    exists M'. *)
+(*    exists K'. *)
+(*    exists f. *)
+(*    * auto. *)
+(*    * assert (H0 : deepest_K (TmBind (TmBind M N) t) = *)
+(*                   let (K0, M0) := deepest_K (TmBind M N) in *)
+(*                   (Iterate t K0, M0)) by auto. *)
+
+(*      rewrite H0 in Hb. *)
+
+(*      pose (X := deepest_K (TmBind M N)). *)
+(*      assert (H : X = deepest_K (TmBind M N)) by auto. *)
+(*      clearbody X. *)
+(*      destruct X. *)
+(*      rewrite <- H in Hb. *)
+(*      simpl in H. *)
+
+(*      pose (X := deepest_K M). *)
+(*      assert (H' : X = deepest_K M) by auto. *)
+(*      clearbody X. *)
+(*      destruct X. *)
+
+(*      rewrite <- H. *)
+
+(*      inversion Hb. *)
+(*      subst. *)
+(*      assert (let (K, body) := deepest_K M in *)
+(*              (Iterate t (Iterate N K), body) = (Iterate t K', M')). *)
+
+(* Qed. *)
+
+Lemma deepest_K_TmNull K :
+  deepest_K (plug K TmNull) = (K, TmNull).
+Proof.
+ pose (X := deepest_K TmNull).
+ assert (X = deepest_K TmNull) by auto.
+ simpl in H.
+ erewrite deepest_K_plug; eauto.
+ simpl.
+ auto.
+Qed.
+
+Lemma unique_plug_null:
+  forall K K',
+    (plug K TmNull = plug K' TmNull) -> K = K'.
+Proof.
+ intros.
+ assert (deepest_K (plug K TmNull) = (K, TmNull)).
+  apply deepest_K_TmNull.
+ assert (deepest_K (plug K' TmNull) = (K', TmNull)).
+  apply deepest_K_TmNull.
+ congruence.
+Qed.
+
+Hint Resolve unique_plug_null.
+
+Lemma Rw_null_Krw:
+  forall K' K,
+    Ksize K = Ksize K' ->
+    (plug K' TmNull ~> plug K TmNull) ->
+    Krw K' K.
+Proof.
+ intros.
+ let T := type of H0 in copy T.
+ apply K_TmNull_rw in H0.
+ destruct H0 as [[K0 [N [Ha Hb]]] | [K0 [Ha Hb]]].
+  subst.
+  assert (K = K0).
+   apply unique_plug_null; auto.
+  subst.
+  simpl in H.
+  exfalso.
+  omega.
+ assert (K = K0).
+  apply unique_plug_null; auto.
+ subst.
+  auto.
+Qed.
+
+Lemma plug_form:
+  forall K M,
+    (plug K M = M) + ({M1 : Term & {N1 : Term & plug K M = TmBind M1 N1}}).
+Proof.
+ induction K; simpl.
+ - left.
+   auto.
+ - right.
+   destruct (IHK (TmBind M t)); eauto.
+Qed.
+
+Lemma Rw_conserves_Ksize:
+  forall K K',
+    (plug K TmNull ~> plug K' TmNull) -> Ksize K >= Ksize K'.
+Proof.
+ induction K.
+  simpl.
+  intros.
+  inversion H.
+ simpl.
+ intros.
+ let T := type of H in assert (H' : T) by auto.
+ apply Neutral_Lists in H; try auto.
+ destruct H as [[M' [Ha Hb]] | [K0 [Ha Hb]]].
+  inversion Hb.
+    subst.
+    assert (K' = K).
+     apply unique_plug_null; sauto.
+    subst.
+    omega.
+   subst.
+   inversion H2.
+  subst.
+  assert (K' = Iterate n' K).
+   apply unique_plug_null.
+   simpl in *; sauto.
+  subst.
+  simpl.
+  omega.
+ assert (K' = Iterate t K0).
+  apply unique_plug_null.
+  simpl in *; sauto.
+ subst.
+ replace (plug K (TmBind TmNull t)) with (plug (Iterate t K) TmNull) in H' by auto.
+ simpl.
+ assert (plug K TmNull ~> plug K0 TmNull).
+  auto.
+ apply IHK in H.
+ omega.
+Qed.
+
+Lemma Krw_rt_conserves_Ksize:
+  forall K K',
+    Krw_rt K K' -> Ksize K >= Ksize K'.
+Proof.
+ intros.
+ induction H.
+   subst; sauto.
+  specialize (k TmNull).
+  apply Rw_conserves_Ksize; sauto.
+ omega.
+Qed.
+
+Lemma rw_rt_preserves_plug_TmNull:
+  forall (x : Continuation) (M N : Term),
+    (M ~>> N) -> {x : Continuation& M = plug x TmNull} -> {y : Continuation & N = plug y TmNull}.
+Proof.
+ intros x M N H H0.
+ induction H.
+ - subst.
+   eauto.
+ - destruct H0.
+   subst.
+   apply K_TmNull_rw in r.
+   destruct r.
+   destruct s.
+   destruct s.
+   destruct p.
+   exists x1; auto.
+   destruct s.
+   destruct p.
+   exists x1; auto.
+ - firstorder.
+Qed.
+
+(* Lemma goofy: *)
+(*   forall K M K', *)
+(*     SN (plug K M) -> (plug K TmNull ~> plug K' TmNull) -> SN (plug K' M). *)
+(* Proof. *)
+(*  intros. *)
+(*  apply SN_embedding2 with (f := fun m => plug K m) *)
+(*                           (g := fun m => plug K' m) *)
+(*                           (Q := plug K M) *)
+(*                           (Q' := plug K' M); try auto. *)
+(*  intros. *)
+
+(* Qed. *)
+
+Inductive prefix : Continuation -> Continuation -> Set :=
+  prefix_refl : forall K, prefix K K
+| prefix_frame :forall K K' N, prefix K' K -> prefix K' (Iterate N K).
+
+Lemma reexamine:
+  forall K' K,
+    prefix K' K
+    -> forall M, {M' : Term & plug K' M' = plug K M}.
+Proof.
+ induction K; simpl; intros.
+  inversion H.
+  subst.
+  simpl.
+  exists M; sauto.
+
+ inversion H.
+  subst.
+  exists M.
+
+   auto.
+
+ subst.
+ pose (IHK H2 (TmBind M t)).
+ destruct s.
+ eauto.
+Qed.
+
+(* Lemma dropoff_lemma: *)
+(*   forall K K', *)
+(*     (plug K TmNull ~>> plug K' TmNull) *)
+(*     -> {K'' : Continuation & (Krw_rt K K'' * *)
+(*         {K''' : Continuation & *)
+(*           ((plug K'' TmNull ~> plug K''' TmNull) * *)
+(*            (Ksize K''' < Ksize K'') * *)
+(*            (plug K''' TmNull ~>> plug K' TmNull))%type})%type}. *)
+(* Proof. *)
+
+(* Qed. *)
+
+Inductive relK : Continuation -> Continuation -> Set :=
+  rw : forall K K', Krw K K' -> relK K K'
+| strip : forall K K' t, K = Iterate t K' -> relK K K'.
+
+Inductive relK_rt  : Continuation -> Continuation -> Set :=
+  refl : forall K, relK_rt K K
+| step : forall K K', relK K K' -> relK_rt K K'
+| trans : forall K K' K'', relK_rt K K' -> relK_rt K' K'' -> relK_rt K K''.
+
+Hint Constructors relK relK_rt.
+
+Lemma magic:
+forall K K',
+  relK_rt K K'
+  -> forall M,
+       SN (plug K M)
+  -> {M' : Term & SN (plug K' M')}.
+Proof.
+ intros K K' rel.
+ induction rel; intros M sn.
+   seauto.
+  destruct r.
+   pose (k M).
+   exists M.
+   inversion sn.
+   seauto.
+  lapply (reexamine K' (Iterate t K')).
+   intros H.
+   subst.
+   specialize (H M).
+   destruct H.
+   exists x.
+   simpl in *.
+   rewrite e.
+   sauto.
+  apply prefix_frame.
+  apply prefix_refl.
+ pose (s := IHrel1 M sn).
+ destruct s.
+ pose (IHrel2 x s).
+ sauto.
+Qed.
+
+Lemma K_TmNull_relK:
+  forall K K',
+    (plug K TmNull ~> plug K' TmNull)
+    -> relK K K'.
+Proof.
+ intros.
+ apply K_TmNull_rw in H.
+ destruct H as [[K_shorter [N [H1a H1b]]] | [K'' [H1a H1b]]].
+  subst.
+  eapply strip.
+  apply unique_plug_null in H1a.
+  subst.
+  eauto.
+  apply rw.
+ apply unique_plug_null in H1b.
+ subst.
+ auto.
+Qed.
+
+Definition is_K_null M := {K : Continuation & M = plug K TmNull}.
+
+Definition gimme_K M (p : is_K_null M) := projT1 p.
+
+Lemma K_TmNull_rw_abstract
+     : forall (K : Continuation) (Z : Term),
+       (plug K TmNull ~> Z) ->
+       {K' : Continuation & Z = plug K' TmNull}.
+Proof.
+intros.
+apply K_TmNull_rw in H.
+destruct H; firstorder.
+Qed.
+
+Lemma K_TmNull_rw_rt:
+  forall A Z,
+    (A ~>> Z) ->
+    is_K_null A -> is_K_null Z.
+Proof.
+ intros.
+ induction H; unfold is_K_null; firstorder; subst.
+  subst.
+  eauto.
+ eauto using K_TmNull_rw_abstract.
+Qed.
+
+Lemma K_TmNull_relK_rt_inner:
+  forall A Z
+    (pA : is_K_null A) (pZ: is_K_null Z),
+    (A ~>> Z) ->
+    relK_rt (gimme_K A pA) (gimme_K Z pZ).
+Proof.
+ intros.
+ induction H; destruct pA; destruct pZ; subst; simpl in *.
+   apply unique_plug_null in e.
+   subst.
+   apply refl.
+  apply step.
+  apply K_TmNull_rw in r.
+  destruct r as [[K' [N [H1a H1b]]] | [K' [H1a H1b]]].
+   subst x.
+   replace x0 with K'.
+    eapply strip; eauto.
+   apply unique_plug_null; auto.
+  apply rw.
+  replace x0 with K'.
+   sauto.
+  apply unique_plug_null; auto.
+ assert (is_K_null (plug x TmNull)).
+  unfold is_K_null.
+  eauto.
+ specialize (IHRewritesTo_rt1 H1).
+ assert (is_K_null m).
+  apply K_TmNull_rw_rt with (A := plug x TmNull); auto.
+ specialize (IHRewritesTo_rt1 H2).
+ replace (gimme_K (plug x TmNull) H1) with x in IHRewritesTo_rt1.
+  apply trans with (gimme_K m H2); auto.
+  assert (H3 : is_K_null (plug x0 TmNull)).
+   unfold is_K_null.
+   eauto.
+  specialize (IHRewritesTo_rt2 H2 H3).
+  replace (gimme_K (plug x0 TmNull) H3) with x0 in IHRewritesTo_rt2.
+   exact IHRewritesTo_rt2.
+  unfold gimme_K.
+  unfold projT1.
+  destruct H3.
+  apply unique_plug_null; auto.
+ unfold gimme_K.
+ unfold projT1.
+ destruct H1.
+ apply unique_plug_null; auto.
+Qed.
+
+Lemma K_TmNull_relK_rt:
+  forall K K',
+    (plug K TmNull ~>> plug K' TmNull)
+    -> relK_rt K K'.
+Proof.
+ intros.
+ assert (is_K_null (plug K TmNull)).
+  unfold is_K_null.
+  eauto.
+ assert (is_K_null (plug K' TmNull)).
+  unfold is_K_null.
+  eauto.
+ eapply K_TmNull_relK_rt_inner in H; eauto.
+ replace (gimme_K (plug K TmNull) H0) with K in H.
+  replace (gimme_K (plug K' TmNull) H1) with K' in H.
+   auto.
+  destruct H1.
+  simpl.
+  auto using unique_plug_null.
+ destruct H0.
+ simpl.
+ auto using unique_plug_null.
+Qed.
+
+Lemma Krw_rt_Rw_rt:
+  forall K K' M, Krw_rt K K' -> (plug K M ~>> plug K' M).
+Proof.
+ intros.
+ induction H; subst; eauto.
+Qed.
+
+Lemma Rw_rt_under_K:
+  forall K M N,
+    (M ~>> N) -> (plug K M ~>> plug K N).
+Proof.
+ intros K M N red.
+ induction red.
+   subst; auto.
+  eauto using Rw_rt_step, Rw_under_K.
+ eauto.
+Qed.
+
+(* (* TODO: Should be able to get "induction on Krw sequences" directly
+      from SN . plug like this: *)
+SN (plug K M) ->
+(forall K0, Krw_rt K K0 -> (forall K', Krw K0 K' -> (P K' -> P K0))) ->
+P K.
+ *)
